Strata/Transform/LoopElim.lean
@@ -29,7 +29,7 @@ def Stmt.removeLoopsM
     let invariant := invariant?.getD HasBool.tt
     let loop_num ← StateT.modifyGet (fun x => (x, x + 1))
     let neg_guard : P.Expr := HasNot.not guard
-    let assigned_vars := Stmts.modifiedVars bss
+    let assigned_vars := Block.modifiedVars bss
     let havocd : Stmt P C :=
       .block s!"loop_havoc_{loop_num}" (assigned_vars.map (λ n => Stmt.cmd (HasHavoc.havoc n))) {}
     let entry_invariant :=
@@ -40,7 +40,7 @@ def Stmt.removeLoopsM
              (Stmt.cmd (HasPassiveCmds.assume s!"assume_invariant_{loop_num}" invariant))]
     let maintain_invariant :=
       Stmt.cmd (HasPassiveCmds.assert s!"arbitrary_iter_maintain_invariant_{loop_num}" invariant)
-    let body_statements ← Stmts.removeLoopsM bss
+    let body_statements ← Block.removeLoopsM bss
     let arbitrary_iter_facts := .block s!"arbitrary_iter_facts_{loop_num}"
       ([havocd, arbitrary_iter_assumes] ++
             body_statements ++
@@ -49,23 +49,23 @@ def Stmt.removeLoopsM
     let invariant := Stmt.cmd (HasPassiveCmds.assume s!"invariant_{loop_num}" invariant)
     pure (.ite guard [first_iter_facts, arbitrary_iter_facts, havocd, not_guard, invariant] [] {})
   | .ite c tss ess md => do
-    let tss ← Stmts.removeLoopsM tss
-    let ess ← Stmts.removeLoopsM ess
+    let tss ← Block.removeLoopsM tss
+    let ess ← Block.removeLoopsM ess
     pure (.ite c tss ess md)
   | .block label bss md => do
-    let bss ← Stmts.removeLoopsM bss
+    let bss ← Block.removeLoopsM bss
     pure (.block label bss md)
   | .cmd _ => pure s
   | .goto _ _ => pure s
 
-def Stmts.removeLoopsM
+def Block.removeLoopsM
   [HasNot P] [HasVarsImp P C] [HasHavoc P C] [HasPassiveCmds P C]
   (ss : List (Stmt P C)) : StateM Nat (List (Stmt P C)) :=
   match ss with
   | [] => pure []
   | s :: ss => do
     let s ← Stmt.removeLoopsM s
-    let ss ← Stmts.removeLoopsM ss
+    let ss ← Block.removeLoopsM ss
     pure (s :: ss)
 
 end
